Try to handle partial application for functions

new/golang/defn/globals.v
@@ -54,8 +54,9 @@ Context `{ffi_syntax}.
 
 Definition func_call_def : val :=
   λ: "pkg_name" "func_name",
+    (λ: "firstArg",
     let: (("varAddrs", "functions"), "typeToMethodSets") := globals.unwrap $ GlobalGet "pkg_name" in
-    globals.unwrap $ alist_lookup "func_name" "functions".
+    (globals.unwrap $ alist_lookup "func_name" "functions") "firstArg").
 Program Definition func_call := sealed @func_call_def.
 Definition func_call_unseal : func_call = _ := seal_eq _.
 
